Phi_System/Fiction_Refinement.thy
@@ -48,12 +48,12 @@ definition Raw_Procedure :: "'ret proc
                         \<Rightarrow> ('ret \<phi>arg \<Rightarrow> resource rel)
                         \<Rightarrow> bool"
     ("\<r>\<a>\<w> \<p>\<r>\<o>\<c> (2_) \<r>\<e>\<f>\<i>\<n>\<e>\<s> _ " [11,11] 10)
-  where "Raw_Procedure f S \<longleftrightarrow> (\<forall>x r. f (r * x) \<subseteq> \<S> (\<lambda>v. { r * y | y. (x,y) \<in> S v }) 0)"
+  where "Raw_Procedure f S \<longleftrightarrow> (\<forall>x r. f (r * x) \<subseteq> LooseState (\<lambda>v. { r * y | y. (x,y) \<in> S v }) 0)"
 
 definition Fictional_Refine :: "'ret proc
                         \<Rightarrow> ('ret \<phi>arg \<Rightarrow> fiction rel)
                         \<Rightarrow> bool"
-  where \<open>Fictional_Refine f S \<longleftrightarrow> (\<forall>x r. f (r * x) \<subseteq> \<S> (\<lambda>v. { r * y | y. (x,y) \<in> S v }) 0)\<close> *)
+  where \<open>Fictional_Refine f S \<longleftrightarrow> (\<forall>x r. f (r * x) \<subseteq> LooseState (\<lambda>v. { r * y | y. (x,y) \<in> S v }) 0)\<close> *)
 
 
 
@@ -175,7 +175,7 @@ private lemma from_fictional_refinement':
 \<Longrightarrow> \<p>\<r>\<o>\<c> f \<lbrace> x \<Ztypecolon> \<phi> Itself \<longmapsto> \<lambda>v. y \<Ztypecolon> \<phi> Itself \<s>\<u>\<b>\<j> y. (x,y) \<in> Rel (Normal v) \<rbrace> \<t>\<h>\<r>\<o>\<w>\<s> (\<lambda>e. y \<Ztypecolon> \<phi> Itself \<s>\<u>\<b>\<j> y. (x,y) \<in> Rel (Abnm e))\<close>
   unfolding \<phi>Procedure_alt Fictional_Forward_Simulation_def atomize_all Valid_Transition_def
   apply (auto simp add: Image_iff subset_iff Bex_def R.basic_fiction_\<I> \<phi>expns Transition_of'_def
-          LooseStateSpec_def split_sum_all INTERP_RES_def interp_split' R.\<r>_valid_split' interp_comp_\<I>
+          LooseState_def split_sum_all INTERP_RES_def interp_split' R.\<r>_valid_split' interp_comp_\<I>
           R.inject_wand_homo inject_wand_homo prj.homo_mult eval_stat_forall split: eval_stat.split)
   subgoal premises prems for r u y v y' rr
     thm prems
