Phi_System/PhiSem_Formalization_Tools2.thy
@@ -183,13 +183,13 @@ lemma "__op_try__"[intro!]:
     apply (cases s; simp; cases x; clarsimp simp add: INTERP_SPEC set_mult_expn ring_distribs)
     subgoal premises prems for a b u v
       using prems(1)[THEN spec[where x=comp], THEN spec[where x=R]]
-      by (metis (no_types, lifting) INTERP_SPEC LooseStateSpec_expn(1) prems(3) prems(6) prems(7) prems(8) prems(9) set_mult_expn)
+      by (metis (no_types, lifting) INTERP_SPEC LooseState_expn(1) prems(3) prems(6) prems(7) prems(8) prems(9) set_mult_expn)
     subgoal premises prems for a b c d u v2 proof -
-      have \<open>Abnormal a b \<in> \<S> (\<lambda>v. INTERP_SPEC (R \<heavy_comma> Y1 v)) (\<lambda>v. INTERP_SPEC (R \<heavy_comma> E v))\<close>
+      have \<open>Abnormal a b \<in> LooseState (\<lambda>v. INTERP_SPEC (R \<heavy_comma> Y1 v)) (\<lambda>v. INTERP_SPEC (R \<heavy_comma> E v))\<close>
         using prems(1)[THEN spec[where x=comp], THEN spec[where x=R]]
         using prems(10) prems(3) prems(7) prems(8) prems(9) by blast
       note this[simplified]
-      then have \<open>Success c d \<in> \<S> (\<lambda>v. INTERP_SPEC (R \<heavy_comma> Y2 v)) (\<lambda>v. INTERP_SPEC (R \<heavy_comma> E2 v))\<close>
+      then have \<open>Success c d \<in> LooseState (\<lambda>v. INTERP_SPEC (R \<heavy_comma> Y2 v)) (\<lambda>v. INTERP_SPEC (R \<heavy_comma> E2 v))\<close>
         using prems(2)[of a, THEN spec[where x=b], THEN spec[where x=R]]
         by (meson INTERP_SPEC prems(4) set_mult_expn)
       note this[simplified]
@@ -197,18 +197,18 @@ lemma "__op_try__"[intro!]:
         by (metis INTERP_SPEC prems(11) set_mult_expn)
     qed
     subgoal premises prems for a b c d u v proof -
-      have \<open>Abnormal a b \<in> \<S> (\<lambda>v. INTERP_SPEC (R \<heavy_comma> Y1 v)) (\<lambda>v. INTERP_SPEC (R \<heavy_comma> E v))\<close>
+      have \<open>Abnormal a b \<in> LooseState (\<lambda>v. INTERP_SPEC (R \<heavy_comma> Y1 v)) (\<lambda>v. INTERP_SPEC (R \<heavy_comma> E v))\<close>
         using prems(1)[THEN spec[where x=comp], THEN spec[where x=R]]
         using prems(10) prems(3) prems(7) prems(8) prems(9) by blast
       note this[simplified]
-      then have \<open>Abnormal c d \<in> \<S> (\<lambda>v. INTERP_SPEC (R \<heavy_comma> Y2 v)) (\<lambda>v. INTERP_SPEC (R \<heavy_comma> E2 v))\<close>
+      then have \<open>Abnormal c d \<in> LooseState (\<lambda>v. INTERP_SPEC (R \<heavy_comma> Y2 v)) (\<lambda>v. INTERP_SPEC (R \<heavy_comma> E2 v))\<close>
         using prems(2)[THEN spec[where x=b], THEN spec[where x=R]]
         by (meson INTERP_SPEC prems(4) set_mult_expn)
       note this[simplified]
       then show ?thesis
         by (simp add: INTERP_SPEC set_mult_expn)
     qed
-     apply (smt (z3) INTERP_SPEC LooseStateSpec_expn(2) LooseStateSpec_expn(3) set_mult_expn)
+     apply (smt (z3) INTERP_SPEC LooseState_expn(2) LooseState_expn(3) set_mult_expn)
     by blast .
 
 definition "Union_the_Same_Or_Arbitrary_when_Var Z X Y \<longleftrightarrow> (\<forall>v. (Z::'v \<Rightarrow> 'a set) v = X v + Y v)"
